Implemented redblackSort, refactored treeSort, added a base file with some tactics common to the other files. Refactored the rebuild script.

Sorting/Heapsort.v
@@ -23,27 +23,27 @@ Function fromList' {A : LinDec} (l : list A) : BTree A :=
   fold_left (fun t x => insert' x t) l empty.
 
 Function toList {A : LinDec} (t : BTree A)
-  {measure len t} : list A :=
+  {measure size t} : list A :=
 match deleteMin t with
     | (None, _) => []
     | (Some m, t') => m :: toList t'
 end.
 Proof.
   destruct t; cbn; inversion 1; inversion 1; subst.
-  rewrite merge'_len. omega.
+  rewrite merge'_size. omega.
 Defined.
 
 Arguments toList [x] _.
 
 Function toList'_aux {A : LinDec} (t : BTree A) (acc : list A)
-  {measure len t} : list A :=
+  {measure size t} : list A :=
 match deleteMin t with
     | (None, _) => acc
     | (Some m, t') => toList'_aux t' (m :: acc)
 end.
 Proof.
   destruct t; cbn; inversion 2; inversion 1; subst.
-  rewrite merge'_len. omega.
+  rewrite merge'_size. omega.
 Defined.
 
 Definition toList' {A : LinDec} (t : BTree A) : list A :=
@@ -53,7 +53,4 @@ Definition leftistHeapsort (A : LinDec) (l : list A)
   : list A := toList (fromList l).
 
 Definition leftistHeapsort' (A : LinDec) (l : list A)
-  : list A := toList' (fromList' l).
-
-Time Compute leftistHeapsort natle (cycle 50 testl).
-Time Compute leftistHeapsort' natle (cycle 50 testl).
+  : list A := rev_append (toList' (fromList' l)) [].
