RCCBase.v
@@ -1,0 +1,61 @@
+Require Export FunctionalExtensionality.
+
+Ltac inv H := inversion H; subst.
+
+Ltac gen x := generalize dependent x.
+
+Ltac ext x := extensionality x.
+
+Ltac term_contains t x :=
+match t with
+    | x => idtac
+    | ?f x => idtac
+    | ?f _ => term_contains f x
+    | _ => fail
+end.
+
+Ltac gen_IH H :=
+match reverse goal with
+    | H : _ |- _ => fail
+    | x : ?Tx |- _ =>
+        match type of H with
+            | ?TH => term_contains TH x
+            | _ => generalize dependent x
+        end
+end.
+
+Ltac gen_ind H :=
+  try intros until H; gen_IH H; induction H; cbn; auto.
+
+
+Ltac invs := repeat
+match goal with
+    | H : ?f ?x1 ?x2 ?x3 = ?f ?x1' ?x2' ?x3' |- _ => inv H
+    | H : ?f ?x1 ?x2 = ?f ?x1' ?x2' |- _ => inv H
+    | H : ?f ?x1 = ?f ?x1' |- _ => inv H
+end.
+
+Ltac replace_nonvars H :=
+match H with
+    | ?f ?x1 => is_var x1; replace_nonvars f
+    | ?f ?x1 =>
+        let x1' := fresh "x1" in
+        let H1 := fresh "H1" in remember x1 as x1' eqn: H1; replace_nonvars f
+    | _ => idtac
+end.
+
+Ltac clean_eqs := repeat
+match goal with
+    | H : ?x = ?x |- _ => clear H
+    | H : ?x = ?x -> _ |- _ => specialize (H eq_refl)
+    | H : forall x, ?y = ?y -> ?P |- _ =>
+        assert (H' := fun x => H x eq_refl); clear H; rename H' into H
+end.
+
+Ltac ind' H :=
+match type of H with
+    | ?T => replace_nonvars T; induction H; subst; try congruence;
+        invs; clean_eqs; eauto
+end.
+
+Ltac ind H := try intros until H; gen_IH H; ind' H.
