Sorting/RedblackSort.v
@@ -1,0 +1,52 @@
+Add Rec LoadPath "/home/zeimer/Code/Coq".
+
+Require Import RedBlack.
+
+Function toList {A : Type} (t : RBTree A) : list A :=
+match t with
+    | E => []
+    | T _ l v r => toList l ++ v :: toList r
+end.
+
+Fixpoint fromList {A : LinDec} (l : list A) : RBTree A :=
+match l with
+    | [] => E
+    | h :: t => ins h (fromList t)
+end.
+
+Fixpoint toList'_aux {A : Type} (t : RBTree A) (acc : list A) : list A :=
+match t with
+    | E => acc
+    | T _ l v r => toList'_aux l (v :: toList'_aux r acc)
+end.
+
+Definition toList' {A : Type} (t : RBTree A) : list A := toList'_aux t [].
+
+Definition fromList' {A : LinDec} (l : list A) : RBTree A :=
+  fold_left (fun t x => ins x t) l E.
+
+Lemma toList'_aux_spec :
+  forall (A : Type) (t : RBTree A) (acc : list A),
+    toList'_aux t acc = toList t ++ acc.
+Proof.
+  induction t; cbn; intros.
+    trivial.
+    rewrite IHt1, IHt2, <- app_assoc, <- app_comm_cons. trivial.
+Qed.
+
+Theorem toList'_spec : @toList' = @toList.
+Proof.
+  ext A. ext t. unfold toList'.
+  rewrite toList'_aux_spec, app_nil_r. trivial.
+Qed.
+
+Definition redblackSort (A : LinDec) (l : list A) : list A :=
+  toList (fromList l).
+
+Definition redblackSort' (A : LinDec) (l : list A) : list A :=
+  toList' (fromList' l).
+
+Require Import ListLemmas.
+
+Time Compute redblackSort natle (cycle 200 testl).
+Time Compute redblackSort' natle (cycle 200 testl).
