Sorting/Test.v
@@ -2,16 +2,21 @@ Add Rec LoadPath "/home/zeimer/Code/Coq".
 
 Require Import InsertionSort.
 Require Import SelectionSort.
-Require Import QuickSort.
-Require Import MergeSort.
-Require Import Heapsort.
 
-Require Import BST.
+Require Import MergeSort.
+Require Import QuickSort.
+
+Require Import TreeSort.
+Require Import Heapsort.
+Require Import RedblackSort.
+
 Require Import ListLemmas.
+
+Require Import TrichQuicksort.
 
 Set Implicit Arguments.
 
-Require Import Coq.Sorting.Heap.
+(*Require Import Coq.Sorting.Heap.
 
 Lemma my_le_trans :
   forall a b c : nat, a <= b -> b <= c -> a <= c.
@@ -19,48 +24,101 @@ Proof.
   induction a as [| a']; simpl; intros.
     omega.
     omega.
-Defined.
+Defined.*)
 
+(* Slow sorts on small lists. *)
+(*Time Compute ss natle (cycle 10 testl).
+Time Compute insertionSort natle (cycle 10 testl).*)
 
-(*Time Compute hms2 128 natle (cycle 100 testl).
-Time Compute ms natle (cycle 100 testl).
+(* Fast sorts on medium lists. *)
+(*Time Compute ms natle (cycle 100 testl).
 Time Compute ms2 natle (cycle 100 testl).
-Time Compute hms 128 natle (cycle 100 testl). *)
 
-(*Time Compute insertionSort natle (cycle 2500 testl).
-Time Compute treeSort natle (cycle 2500 testl).*)
+Time Compute qs natle (cycle 100 testl).
+Time Compute qs2 natle (cycle 100 testl).
 
-(*Time Compute leftistHeapsort natle (cycle 1 testl).
+Time Compute tqs natlt (cycle 100 testl).
 
-Time Compute qs natle (cycle 5 testl).
-Time Compute qs2 natle (cycle 5 testl).
-
-Time Compute insertionSort natle (cycle 5 testl).
-Time Compute ss natle (cycle 5 testl).
-
-Time Compute leftistHeapsort natle (cycle 2 testl).
-
-Time Compute hqs 2048 natle (cycle 750 testl).
-Time Compute hqs2 2048 natle (treeSort natle) (cycle 750 testl).
-Time Compute treeSort natle (cycle 750 testl).
-Time Compute hqs2 16 natle (leftistHeapsort natle) (cycle 100 testl).
-Time Compute hms 1024 natle (cycle 100 testl).
 Time Compute treeSort natle (cycle 100 testl).
-Time Compute leftistHeapsort natle (cycle 20 testl).
+Time Compute treeSort' natle (cycle 100 testl).
 
-Time Compute hqs 1024 natle (cycle 2000 [1]).
-Time Compute hms 1024 natle (cycle 2000 [1]).
-Time Compute treeSort natle (cycle 2000 [1]).*)
+Time Compute redblackSort natle (cycle 100 testl).
+Time Compute redblackSort' natle (cycle 100 testl).
 
-(*Time Compute ms natle (cycle 3000 wut).
-Time Compute qs natle (cycle 3000 wut).*)
+Time Eval lazy in leftistHeapsort natle (cycle 100 testl).
+Time Eval lazy in leftistHeapsort' natle (cycle 100 testl).*)
 
-Require Import TrichQuicksort.
-Require Import TrichDec.
+(* Fast sorts on big lists. *)
+(*Time Compute ms natle (cycle 200 testl).
+Time Compute ms2 natle (cycle 200 testl).
 
-Definition wut := [1].
+Time Compute qs natle (cycle 200 testl).
+Time Compute qs2 natle (cycle 200 testl).*)
 
-Time Compute tqs natlt (cycle 3000 wut).
+(*Time Compute tqs natlt (cycle 1000 testl).
+
+Time Compute treeSort natle (cycle 1000 testl).
+Time Compute treeSort' natle (cycle 1000 testl).
+
+Time Compute redblackSort natle (cycle 1000 testl).
+Time Compute redblackSort' natle (cycle 1000 testl).
+
+Time Eval lazy in leftistHeapsort' natle (cycle 300 testl).*)
+
+(* Hybrid mergesort on big lists. *)
+(*Time Compute @ghms 512 natle (insertionSort natle) (MsSplit natle)
+  (cycle 200 testl).
+
+Time Compute @ghms 1024 natle (treeSort natle) (MsSplit natle)
+  (cycle 200 testl).
+
+Time Compute @ghms 1024 natle (redblackSort natle) (MsSplit natle)
+  (cycle 200 testl). *)
+
+(* Bad
+Time Compute @ghms 1024 natle (leftistHeapsort' natle) (MsSplit natle)
+  (cycle 200 testl).
+*)
+
+(*Time Compute @hqs 1024 natle (insertionSort natle) (cycle 200 testl).
+
+Time Compute @hqs 512 natle (treeSort natle) (cycle 200 testl).
+
+Time Compute @hqs 512 natle (redblackSort natle) (cycle 200 testl).
+*)
+
+(* Bad
+  Time Compute @hqs 256 natle (leftistHeapsort natle) (cycle 200 testl).
+*)
+
+(*Time Compute @htqs 1 natlt (insertionSort natle) (cycle 200 testl).
+
+Time Compute @htqs 1 natlt (treeSort natle) (cycle 200 testl).
+
+Time Compute @htqs 1 natlt (redblackSort natle) (cycle 200 testl).*)
+
+(* Long lists made of one element. *)
+Definition l1 := cycle 2500 [0].
+
+(*Time Compute @ghms 64 natle (insertionSort natle) (MsSplit natle) l1.
+
+Time Compute @ghms 64 natle (treeSort natle) (MsSplit natle) l1.
+
+Time Compute @ghms 64 natle (redblackSort natle) (MsSplit natle) l1.
+
+Time Compute @ghms 64 natle (leftistHeapsort' natle) (MsSplit natle) l1.
+
+Time Compute @hqs 1024 natle (insertionSort natle) l1.
+
+Time Compute @hqs 512 natle (treeSort natle) l1.
+
+Time Compute @hqs 512 natle (redblackSort natle) l1.
+
+Time Compute @htqs 0 natlt (insertionSort natle) l1.
+
+Time Compute @htqs 0 natlt (treeSort natle) l1.
+
+Time Compute @htqs 0 natlt (redblackSort natle) l1.*)
 
 Fixpoint toN (n : nat) : list nat :=
 match n with
@@ -71,12 +129,8 @@ end.
 (*CoFixpoint rand (seed n1 n2 : Z) : Stream Z :=
 let seed' := Zmod seed n2 in Cons seed' (rand (seed' * n1) n1 n2).*)
 
-Require Import RedBlack.
-
 Time Compute qs natle (toN 200).
 Time Compute tqs natlt (toN 200).
-Time Compute insertionSort natle (toN 150).
-Time Compute redblackSort natle (toN 150).
-
-Time Compute htqs 1024 natlt (insertionSort natle) (cycle 500 testl).
-Time Compute htqs 256 natlt (redblackSort natle) (cycle 500 testl).
+Time Compute insertionSort natle (toN 500).
+Time Compute treeSort natle (toN 500).
+Time Compute redblackSort natle (toN 500).
