Sorting/TreeSort.v
@@ -1,0 +1,19 @@
+Add Rec LoadPath "/home/zeimer/Code/Coq".
+
+Require Export LinDec.
+Require Export Sorting.Sort.
+
+Require Export BTree.
+Require Export BST.
+
+Require Export ListLemmas.
+
+Definition treeSort (A : LinDec) (l : list A) : list A :=
+  toList (fromList A l).
+
+Definition treeSort' (A : LinDec) (l : list A) : list A :=
+  toList' (fromList' l).
+
+Time Compute treeSort natle (cycle 100 testl).
+Time Compute treeSort' natle (cycle 100 testl).
+  
