Sorting/TreeSortSpec.v
@@ -1,0 +1,34 @@
+Add Rec LoadPath "/home/zeimer/Code/Coq".
+
+Require Import TreeSort.
+
+From mathcomp Require Import ssreflect.
+
+Theorem treeSort_sorted :
+  forall (A : LinDec) (l : list A), sorted A (treeSort A l).
+Proof.
+  unfold treeSort. intros. apply toList_sorted. apply fromList_is_bst.
+Qed.
+
+Theorem treeSort_perm :
+  forall (A : LinDec) (l : list A),
+    perm A l (treeSort A l).
+Proof.
+  unfold treeSort, perm. intros.
+  elim: l => [| h t IH] //=.
+    by rewrite count_toList count_ins -count_toList -IH.
+Qed.
+
+Instance Sort_treeSort : Sort :=
+{
+    sort := treeSort;
+    sort_sorted := treeSort_sorted;
+    sort_perm := treeSort_perm
+}.
+
+Theorem treeSort'_sorted :
+  forall (A : LinDec) (l : list A), sorted A (treeSort' A l).
+Proof.
+  unfold treeSort'. intros. apply toList'_sorted.
+  try apply fromList'_is_bst.
+Abort.
