new_rebuild.sh
@@ -1,4 +1,0 @@
-#!/bin/bash
-./clean.sh
-./make_makefile.sh
-make
