rebuild.sh
@@ -1,5 +1,4 @@
-#!/bin/sh
-
-make clean
+#!/bin/bash
+./clean.sh
 ./make_makefile.sh
 make
